

$$ D' = \dfrac{D \cdot L}{L - t - r + \sqrt{r^2 - \left(\dfrac{D}{2}\right)^2}} = \dfrac{D \cdot L}{k} $$
$$ \dfrac{\partial D'}{\partial D} = \dfrac{L}{k} - (D \cdot L)\left(\dfrac{-D}{4k^2\sqrt{r^2 - \left(\dfrac{D}{2}\right)^2}}\right) $$
$$ \dfrac{\partial D'}{\partial L} = \dfrac{D}{k} - \dfrac{D \cdot L}{k^2} $$

$$ k = \dfrac{D \cdot L}{D'} $$
$$ \dfrac{\partial D'}{\partial D} = \dfrac{D'}{D} + \left(\dfrac{(D')^2}{4L\sqrt{r^2 - \left(\dfrac{D}{2}\right)^2}}\right) $$
$$ \dfrac{\partial D'}{\partial L} = \dfrac{D'}{L} - \dfrac{(D')^2}{D L} $$

