$$P(s) = \dfrac{e^{-\tfrac{E(s)}{k_bT}}}{Z} \ \ \ \ \ Z = \displaystyle\sum_s e^{-\tfrac{E(s)}{k_bT}}$$
$$\braket{E} = \displaystyle\sum_s E(s)P(s)$$
$$\braket{E}=-\dfrac{1}{Z}\dfrac{\partial Z}{\partial \beta} \ \ \ \ \ \beta = \dfrac{1}{k_bT}$$
$$\braket{E^2}=-\dfrac{1}{Z}\dfrac{\partial^2 Z}{\partial \beta^2} \ \ \ \ \ \beta = \dfrac{1}{k_bT}$$

### Example: Paramagnets
Note: $\mu B = E(\text{state})$.
$$Z = e^{-\beta(-\mu B)}+ e^{-\beta(+\mu B)} = 2\cosh(\beta\mu B)$$
$$\dfrac{d\braket{E}}{dN} = -\dfrac{1}{Z}\dfrac{\partial Z}{\partial \beta} = -\mu B \tanh(\beta\mu B)$$
$$\braket{E} = -N \mu B \tanh(\beta\mu B)$$

